cfrontend/Locally.v
@@ -5,7 +5,7 @@ Export Maps.PTree.
 Notation "a ! b" := (get b a) (at level 1).
 
 Definition hlocally {A} (le : t A) (f : t A -> iProp) : hprop :=
-  fun h => forall le', (forall id, In id h -> le ! id = le' ! id) -> f le' () h.
+  fun h => forall le', (forall id v, h !! id = Some v -> le ! id = le' ! id) -> f le' () h.
 
 Definition locally {A} (le : t A) (f : t A -> iProp) : iProp := MonPred (fun _ => hlocally le f) _.
 
@@ -15,9 +15,9 @@ Ltac inv H := inversion H; clear H; subst.
 
 Ltac unfold_locally :=
 unfold locally; unfold hlocally; MonPred.unseal; split; MonPred.unseal; intros i h H;
-    destruct i; inv H; repeat red; intros a b; destruct a; clear b; exists emp, nil, nil;
-      repeat split; auto; [intros h H0; inversion_star h H; clear H0; inversion H1; subst; simpl in *
-                          | intros x y P0 P1; inversion P0].
+    destruct i; inv H; repeat red; intros a b; destruct a; clear b;
+  exists emp, heap_empty, heap_empty; repeat split; auto; [intros h H0; inversion_star h H; clear H0; inversion H1; subst; simpl in *; rewrite heap_union_empty_l
+                                                     | rewrite heap_union_empty_l; auto ].
 
 Lemma locally_base {A} : forall (le : t A), ⊢ locally le (fun le' => emp).
 Proof.
@@ -27,27 +27,21 @@ Qed.
 
 Lemma locally_elim {A} : forall P (le : t A), ⊢ locally le (fun le' => P le') -∗ P le.
 Proof.
-  unfold_locally.
-  eapply prop_eq; eauto. apply list_eq_comm. auto.
+  unfold_locally. apply H2. intros. auto.
 Qed.
 
 Lemma locally_consequence {A} : forall (P Q : t A -> iProp) (le : t A),
     ⊢locally le (λ le', P le') -∗ (∀ le, P le -∗ Q le) -∗ locally le (λ le', Q le').
 Proof.
   unfold_locally. clear H3. intros j P0. destruct j. clear P0.
-  repeat red. exists (hheap_ctx h), h, nil. repeat split; auto.
-  red. intros. inversion_star h P. clear H0. red in P1. subst.
+  repeat red. exists (hheap_ctx h1), h1, ∅. repeat split; auto.
+  red. intros. inversion_star h P. clear H. red in P1. subst.
   edestruct P2. reflexivity. inversion_star h P.
-  clear H0. destruct P6. inv H4. clear P7. rewrite app_nil_r in P4.
-  apply H0. exists h3, h0. repeat split; auto. eapply prop_eq; eauto. apply list_eq_comm. eauto.
-  eapply prop_eq. apply list_eq_comm. eauto. eapply H2. intros. erewrite <- H3; auto.
-  apply P0. apply in_or_app. left. apply P1. apply H; auto.
-  eapply list_eq_disjoint. apply list_eq_comm. eauto. apply list_disjoint_comm. auto.
-  intros. apply P0 in H4. apply in_app_or in H4. destruct H4; apply in_or_app.
-  right; auto. left; auto. apply P4; auto. intros. apply P0. apply in_app_or in H4.
-  destruct H4; apply in_or_app; auto. right. apply P4; auto.
-  intros x y P0 P1. inversion P1.
-  all : rewrite <- app_nil_end; auto.
+  clear H. destruct P4. inv H3. clear P5. rewrite heap_union_empty_r.
+  rewrite heap_union_empty_r in P3 P2 H0. apply H.
+  exists h, h1. repeat split; auto. apply H2. intros. eapply H0. rewrite lookup_union_Some_raw.
+  left; eauto. rewrite map_union_comm; auto. rewrite !map_disjoint_spec. intros. inversion H0.
+  rewrite heap_union_empty_r. eauto.
 Qed.
 
 Lemma locally_consequence_2 {A} : forall P Q (le : t A),
@@ -61,19 +55,14 @@ Lemma locally_sep {A} : forall P R (le : t A),
             locally le (fun le' => P le' ∗ R le').
 Proof.
   unfold_locally. intros j P0. destruct j. clear P0 H3 H1.
-  exists (hheap_ctx h), h, nil. repeat split; auto.
-  repeat red. intros. inversion_star h P. clear H0. red in P1. subst.
-  exists h1, h2. repeat split; auto. apply H2.
-  intros. eapply H1. apply P0. apply in_or_app. left. apply P1. apply H; auto.
-  apply P2. intros. apply H1. apply P0. apply in_or_app. right. auto.
-  eapply list_eq_disjoint; eauto. apply list_eq_comm. intro. split; intro.
-  apply H. apply P1; auto. apply P1. apply H; auto.
-  intros. apply P0 in H0. apply in_app_or in H0. destruct H0; apply in_or_app.
-  left. apply H; auto. apply P1; auto. right; auto.
-  intros. apply P0. apply in_app_or in H0. destruct H0; apply in_or_app.
-  left. apply P1. apply H; auto. right; auto.
-  intros x y P0 P1. inversion P1.
-  all : rewrite <- app_nil_end; auto.
+  exists (hheap_ctx h1), h1, heap_empty. repeat split; auto.
+  repeat red. intros. inversion_star h P. clear H. red in P1. subst.
+  exists h1, h0. repeat split; auto. apply H2.
+  intros. eapply H0. rewrite lookup_union_Some_raw. left; eauto.
+  apply P2. intros. eapply H0. rewrite lookup_union_Some_raw. right; eauto.
+  split; eauto. eapply map_disjoint_Some_r; eauto.
+  rewrite !map_disjoint_spec. intros. inversion H0.
+  rewrite heap_union_empty_r. eauto.
 Qed.
 
 Lemma locally_and {A} : forall P R (le : t A),
@@ -82,12 +71,12 @@ Lemma locally_and {A} : forall P R (le : t A),
 Proof.
   unfold locally; unfold hlocally; MonPred.unseal; split; MonPred.unseal; intros i h H;
   destruct i; inversion H as (H0); clear H; subst. intros j H; destruct j; clear H.
-  exists emp, nil, nil; repeat split; auto.
-  3 : intros x y P0 P1; inversion P0.
-  1-2 :inversion_star h P; clear H;
-    destruct P2; inv P1; clear P3; simpl in *; apply list_eq_comm in P0; eapply prop_eq; eauto.
-  apply H. intros. apply H0. apply P0. auto.
-  apply H1. intros. apply H0. apply P0. auto.
+  exists emp, heap_empty, heap_empty; repeat split; auto.
+  3 : rewrite heap_union_empty_l; auto.
+  1-2 :inversion_star h P; clear H; destruct P2; inv P1; clear P3; simpl in *;
+    rewrite heap_union_empty_l; rewrite heap_union_empty_l in H0.
+  apply H. intros. eapply H0. eauto.
+  apply H1. intros. eapply H0. eauto.
 Qed.
 
 Lemma locally_simpl {A} : forall P (le : t A), ⊢(∀ le', P le') -∗ locally le (fun le' => P le').
@@ -111,19 +100,16 @@ Qed.
 Lemma locally_modout {A} : forall P (le : t A),
     ⊢<absorb> (locally le (fun le' => P le')) -∗ locally le (fun le' => <absorb> P le').
 Proof.
-  unfold_locally. clear H3. red in H2. inversion_star h P. clear H2.
-  exists h0, h2. repeat split; auto. apply P2. intros. eapply H0. apply H. apply P0.
-  apply in_or_app. right; auto.
-  intros. apply H in H2. apply P0 in H2. auto.
-  intros. apply H. apply P0. auto.
+  unfold_locally. clear H3. red in H2. inversion_star h P. clear H2. intros.
+  exists h, h0. repeat split; auto. apply P2. intros. eapply H. rewrite P0.
+  rewrite lookup_union_Some_raw. right; auto. split; eauto.
+  eapply map_disjoint_Some_r; eauto.
 Qed.
 
 Lemma locally_idempotence {A} : forall P (le : t A),
     ⊢locally le (fun le' => P le') -∗ locally le (fun le' => locally le' (fun le'' => P le'')).
 Proof.
-  unfold_locally. intros. eapply prop_eq. apply list_eq_comm. eauto. apply H2.
-  intros. apply H in H5. pose H5. apply H0 in i. apply H4 in H5.
-  etransitivity; eauto.
+  unfold_locally. intros. eapply H2. intros. erewrite H; eauto.
 Qed.
 
 Lemma locally_sep_indep_r {A} : forall P Q (le : t A),
@@ -141,15 +127,13 @@ Qed.
 Lemma locally_forall {A B} : forall P (le : t A),
     ⊢(∀ l, locally le (fun le' => P l le')) -∗ locally le (fun le' => ∀ (l:B), P l le').
 Proof.
-  unfold_locally. red. intros. red in H2. eapply prop_eq.
-  apply list_eq_comm. eauto. apply H2. intros. apply H0. apply H; auto.
+  unfold_locally. red. intros. apply H2. auto.
 Qed.
 
 Lemma locally_exists' {A B} : forall P (le : t A),
       ⊢(∃ t, locally le (fun le' => P t le')) -∗ locally le (fun le' => ∃ (t : B), P t le').
 Proof.
-  unfold_locally. intros. clear H3. destruct H2. repeat red. exists x.
-  eapply prop_eq. apply list_eq_comm. eauto. apply H2. intros. apply H0. apply H; auto.
+  unfold_locally. intros. clear H3. destruct H2. repeat red. exists x. apply H0; auto.
 Qed.
 
 Lemma locally_exists {A B} : forall P (le : t A), ∀ t,
@@ -204,20 +188,22 @@ Qed.
 Lemma locally_set {A} : forall Q (le : t A) t v,
     ⊢ & t -∗ locally le (fun le' => Q le') -∗ locally (set t v le) (fun le' => Q le') ∗ & t.
 Proof.
-  unfold_locally. red in H2. clear H3 H1. subst. repeat red. intros. destruct a. clear H0.
-  exists (hheap_ctx h), h, nil. split; auto. repeat split; auto.
-  split. split. intros l H0. inversion_star h P. clear H0. red in P0. exists h2, h0. split.
-  intros le' P3. eapply P1. intros. erewrite <- P3. assert (id <> t0). intro. subst.
-  eapply P2 in H0; eauto. apply P0. apply H. apply H2. apply in_eq. rewrite gso; auto. auto.
-  split; auto. eapply list_eq_trans; eauto. eapply list_eq_trans; eauto.
-  split. apply list_disjoint_comm; auto. apply list_eq_union_comm. auto.
-  reflexivity. split. apply list_disjoint_empty_r. simpl_list. split; auto.
+  unfold_locally. red in H2. clear H3 H1. subst. repeat red. intros. destruct a. clear H.
+  exists (hsingle t0). do 2 eexists. split; auto. reflexivity. repeat split; auto.
+  intros h P. inversion_star h P. clear P. red in P1. subst. exists h1. eexists. split.
+  intros le' P4. eapply P2. intros. erewrite <- P4. assert (id <> t0). intro. subst.
+  eapply map_disjoint_spec; eauto. rewrite lookup_singleton. eauto.
+  rewrite gso; eauto. eauto.
+  repeat split; auto. rewrite map_union_comm; auto.
+  rewrite !map_disjoint_spec. intros. inversion H0.
+  rewrite heap_union_empty_r. eauto.
 Qed.
 
 Lemma locally_lookup {A} : forall le t (v : A),
     ⊢ & t -∗ locally (set t v le) (λ le', ⌜le' ! t = Some v⌝).
 Proof.
-  unfold_locally. intros. red. erewrite <- H0. apply gss. rewrite H. apply H2. apply in_eq.
+  unfold_locally. intros. red. erewrite <- H. apply gss. rewrite H2. rewrite lookup_singleton.
+  eauto.
 Qed.
 
 Lemma locally_out {A} : forall P Q (le : t A),
