cfrontend/SepSet.v
@@ -1,0 +1,370 @@
+Require Import FunctionalExtensionality.
+
+From iris Require Export bi.bi proofmode.tactics proofmode.monpred.
+
+From stdpp Require Export gmap.
+
+Axiom prop_extensionality : forall A B:Prop, (A <-> B) -> A = B.
+Definition pred_incl {A} (P Q : A -> Prop) := forall x, P x -> Q x.
+
+Definition pred_impl {A} (P Q : A -> Prop) := fun x => P x -> Q x.
+
+Notation "P ==> Q" := (pred_incl P Q).
+
+Section hprop.
+  Context {X : Type}.
+  Context {eqX : EqDecision X}.
+  Context {count_X : Countable X}.
+
+  Definition heap : Type := gmap X unit.
+
+  (* Properties on heap *)
+  Instance heap_union_empty_l : LeftId (=@{heap}) ∅ (∪) := _.
+  Instance heap_union_empty_r : RightId (=@{heap}) ∅ (∪) := _.
+  Instance heap_union_assoc : base.Assoc (=@{heap}) (∪).
+  Proof.
+    intros m1 m2 m3. unfold base.union, map_union, union_with, map_union_with.
+    apply (merge_assoc _). intros i.
+    unfold heap in m1. unfold heap in m2. unfold heap in m3.
+      by destruct (m1 !! i), (m2 !! i), (m3 !! i).
+  Qed.
+
+  Definition heap_union_comm (h1 h2 : heap) := map_union_comm h1 h2.
+
+  Lemma heap_disjoint_union_l_l : forall (h1 h2 h3 :heap) , h1 ∪ h2 ##ₘ h3 -> h1 ##ₘ h3.
+  Proof.
+    intros. apply map_disjoint_union_l in H as (P0&P1). assumption.
+  Qed.
+
+  Lemma heap_disjoint_union_l_r : forall (h1 h2 h3 :heap) , h1 ∪ h2 ##ₘ h3 -> h2 ##ₘ h3.
+  Proof.
+    intros. apply map_disjoint_union_l in H as (P0&P1). assumption.
+  Qed.
+
+  Lemma heap_disjoint_union_r_r : forall (h1 h2 h3 :heap) , h1 ##ₘ h2 ∪ h3 -> h1 ##ₘ h3.
+  Proof.
+    intros. apply map_disjoint_union_r in H as (P0&P1). assumption.
+  Qed.
+
+  Lemma heap_disjoint_union_r_l : forall (h1 h2 h3 :heap) , h1 ##ₘ h2 ∪ h3 -> h1 ##ₘ h2.
+  Proof.
+    intros. apply map_disjoint_union_r in H as (P0&P1). assumption.
+  Qed.
+
+  (* Operators *)
+
+  Definition hprop := heap -> Prop.
+
+  Definition hand (H1 H2 : hprop) : hprop :=
+    fun h => H1 h /\ H2 h.
+
+  Definition hor (H1 H2 : hprop) : hprop := fun h => H1 h \/ H2 h.
+
+  Definition hempty : hprop := fun h => h = ∅.
+
+  Definition hsingle l : hprop :=
+    fun h =>  h = {[l := tt]}.
+
+  Definition hheap_ctx (ctx : heap) : hprop := fun h => h = ctx.
+
+  Definition hstar (H1 H2 : hprop) : hprop :=
+    fun h => exists h1 h2, H1 h1 /\ H2 h2 /\ (h1 ##ₘ h2) /\ h = h1 ∪ h2.
+
+  Definition hexists {A} (J : A -> hprop) : hprop := fun h => exists x, J x h.
+  Definition hforall {A} (f : A -> hprop) : hprop := fun h => forall a, f a h.
+
+  Definition hpure (P : Prop) : hprop := fun _ => P.
+
+  Definition hpure_aff (P:Prop) : hprop := fun h => P /\ hempty h.
+
+  Definition htop : hprop := fun h => True.
+
+  Definition hwand (H1 H2 : hprop) : hprop :=
+    hexists (fun (H:hprop) => (hstar H (hpure_aff ((hstar H H1) ==> H2)))).
+
+  Definition qwand A (Q1 Q2:A->hprop) :=
+    hforall (fun x => hwand (Q1 x) (Q2 x)).
+
+  Lemma hempty_intro : hempty ∅.
+  Proof using. reflexivity. Qed.
+
+  Local Notation "'heap_empty'" := (∅ : heap).
+
+  Local Notation "h1 \u h2" := (h1 ∪ h2) (at level 37, right associativity).
+
+  Local Notation "'Hexists' x1 , H" := (hexists (fun x1 => H))
+                                         (at level 39, x1 name, H at level 50).
+  Local Notation "'Hexists' x1 x2 , H" := (Hexists x1, Hexists x2, H)
+                                            (at level 39, x1 name, x2 name, H at level 50).
+  Local Notation "'Hexists' x1 x2 x3 , H" := (Hexists x1, Hexists x2, Hexists x3, H)
+                                               (at level 39, x1 name, x2 name, x3 name, H at level 50).
+
+
+  Local Notation "'\[]'" := (hempty)
+                              (at level 0).
+
+  Local Notation "\[ P ]" := (hpure P)
+                               (at level 0, P at level 99, format "\[ P ]").
+
+  Local Notation "H1 '\*' H2" := (hstar H1 H2)
+                                   (at level 41, right associativity).
+
+  Local Notation "\Top" := htop.
+
+
+  Declare Scope heap_scope.
+
+  Hint Resolve heap_union_empty_l heap_union_empty_r hempty_intro map_disjoint_empty_l map_disjoint_empty_r heap_union_assoc heap_disjoint_union_r_l heap_disjoint_union_l_l heap_disjoint_union_r_r heap_disjoint_union_l_r : heap_scope.
+
+  Ltac inversion_star h P :=
+    match goal with
+    | H : (_ \* _) _ |- _ =>
+      let W := fresh h in
+      let w := fresh P in
+      inversion H as (W&w);
+      let W := fresh h in
+      destruct w as (W&w);
+      do 3 (let w0 := fresh P in
+            destruct w as (w0&w))
+    end.
+  Ltac extens := apply functional_extensionality; intro; apply prop_extensionality.
+
+  Section Properties.
+
+    Lemma hstar_comm : forall H1 H2,
+      H1 \* H2 = H2 \* H1.
+    Proof using.
+      intros H1 H2. extens.
+      split; intro P; inversion_star h P; exists h0; exists h; repeat split; auto;
+        rewrite heap_union_comm; auto.
+    Qed.
+
+    Lemma hstar_assoc : forall H1 H2 H3,
+        (H1 \* H2) \* H3 = H1 \* (H2 \* H3).
+    Proof using.
+      intros H1 H2 H3. extens. split.
+      { intros (h'&h3&(h1&h2&M3&M4&D'&U')&M2&D&U). subst h'.
+        exists h1; exists (h2 ∪ h3). repeat split; auto.
+        { exists h2; exists h3; eauto with heap_scope. }
+        { apply map_disjoint_union_l in D as (P0&P1).
+          apply map_disjoint_union_r. split; auto. }
+        { by rewrite heap_union_assoc. }}
+      { intros (h1&h'&M1&(h2&h3&M3&M4&D'&U')&D&U). subst h'.
+        exists (h1 ∪ h2); exists h3. repeat split; auto.
+        { exists h1; exists h2; eauto with heap_scope. }
+        { rewrite map_disjoint_union_l. split; auto.
+          apply map_disjoint_union_r in D as (P0&P1).
+          assumption. }
+          by rewrite <- heap_union_assoc. }
+    Qed.
+
+  End Properties.
+
+  Definition hpersistent (H:hprop) : hprop := fun h => H heap_empty.
+
+  Definition hlater (H : hprop) := H.
+
+  Set Warnings "-redundant-canonical-projection -convert_concl_no_check".
+  Canonical Structure hpropO := leibnizO hprop.
+
+  Program Canonical Structure hpropI : bi :=
+    Bi hprop _ _ pred_incl hempty hpure hand hor
+       pred_impl (@hforall) (@hexists) hstar hwand hpersistent hlater _ _ _ _.
+  Next Obligation.
+    repeat split; try(solve_proper); eauto.
+    - intros H h P. assumption.
+    - rewrite /Transitive. intros. intros h P. eauto.
+    - rewrite leibniz_equiv_iff. intros (P0&P1). extens. split; intro; auto.
+    - intros n P0 P1 Z. rewrite /hpure. repeat red. extens. auto.
+    - intros n P0 P1 Z. rewrite /hforall. repeat red. intros. extens.
+      split; intros; repeat red in H; apply functional_extensionality in H; subst; auto.
+    - intros n P0 P1 Z. rewrite /hexists. repeat red. intros. extens.
+      split; intro; repeat red in H; apply functional_extensionality in H; subst; auto.
+    - rewrite /hpure. intros φ P imp h P0. apply imp; auto.
+    - rewrite /hand. intros P Q h (P0&P1). apply P0.
+    - rewrite /hand. intros P Q h (P0&P1). apply P1.
+    - rewrite /hor. intros P Q h P0. auto.
+    - rewrite /hor. intros P Q h P0. auto.
+    - rewrite /hor. intros P Q h P0 P1 h0 P2. destruct P2; auto.
+    - intros P Q R P0 h P2 P3. apply P0. split; auto.
+    - intros P Q R P0 h P2. destruct P2. apply P0 in H. apply H in H0. auto.
+    - intros x W a H h P h0. apply H. apply P.
+    - intros h Q a H H0. apply H0.
+    - intros x W H P Q. exists H. apply Q.
+    - intros x W Q P h P0. destruct P0. eapply P. apply H.
+    - intros P P' Q Q' A B C D. inversion_star h P. exists h; exists h0. repeat split; auto.
+    - intros x W A. exists heap_empty; exists W. repeat split; auto with heap_scope.
+      apply map_disjoint_empty_l.
+    - intros P h Q. inversion_star H H. inversion H3. subst.
+      rewrite heap_union_empty_l. apply H4.
+    - intros P Q h R. inversion_star H H. exists H2; exists H0. repeat split; auto. subst.
+      apply heap_union_comm. apply H5.
+    - intros P Q R h P0. rewrite <- hstar_assoc. apply P0.
+    - intros P Q R P0 h P1. exists P. exists h; exists heap_empty. repeat split; auto with heap_scope.
+      apply map_disjoint_empty_r.
+    - intros P Q R W h P0. inversion_star h P. apply W in P2. destruct P2. inversion_star h H.
+      inversion H2. apply H4. exists h2; exists h1. repeat split; auto; subst.
+      + apply heap_disjoint_union_l_l in P4. apply P4.
+      + inversion H5. subst. rewrite heap_union_empty_r. reflexivity.
+    - rewrite /hpersistent. intros P Q H h P0. apply H. apply P0.
+    - rewrite /hpersistent. rewrite /hforall. intros A B C D E. apply D.
+    - rewrite /hpersistent. intros P Q h P0. inversion_star h P. apply P2.
+    - intros P Q x W. destruct W. exists heap_empty; exists x. repeat split; auto with heap_scope.
+      apply map_disjoint_empty_l.
+  Qed.
+  Next Obligation.
+    repeat split; try(solve_proper); eauto.
+    - intros A Φ h a. rewrite /hlater. unfold hforall in *. unfold hlater in a. apply a.
+    - intros A Φ h a. rewrite /hor. unfold hlater in *. destruct a. right. exists x. apply H.
+    - intros Hp h P. unfold hlater in *. right. intro. apply P.
+  Qed.
+
+  Instance inhabited_unit : Inhabited unit.
+  Proof.
+    split. apply ().
+  Qed.
+
+  Instance PreOrder_unit : PreOrder (fun (t1 t2 : unit) => t1 = t2).
+  Proof.
+    split; repeat red; intros; trivial. destruct x,y,z. reflexivity.
+  Qed.
+
+  Program Canonical Structure biInd := BiIndex unit inhabited_unit _ PreOrder_unit.
+
+  Definition single (l : X) : @monPred biInd hpropI := MonPred (fun _ => hsingle l) _.
+
+  Definition heap_ctx (h : heap) : monPred biInd hpropI := MonPred (fun _ => hheap_ctx h) _.
+
+  Ltac inv H := inversion H; clear H; subst.
+
+  Local Open Scope bi_scope.
+
+  Local Notation "'&&' l" :=
+    (heap_ctx l) (at level 20) : bi_scope.
+
+  Local Notation "'&' l" :=
+    (single l) (at level 20) : bi_scope.
+
+  Lemma singleton_neq : forall l l', ⊢ & l -∗ & l' -∗ ⌜l ≠ l'⌝.
+  Proof.
+    MonPred.unseal. split. MonPred.unseal. repeat red. intros. destruct i. destruct a. clear H0.
+    inv H. exists emp, heap_empty, heap_empty. repeat split; auto with heap_scope.
+    intros h H j C. clear C. clear j. inversion_star h P. clear H. inv P0. clear P2.
+    red in P1. rewrite heap_union_empty_l. exists (hheap_ctx h1), h1, heap_empty.
+    repeat split; eauto with heap_scope. subst. intros h H eq. inversion_star h P. clear H.
+    red in P1. red in P0. subst. erewrite map_disjoint_spec in P2.
+    edestruct P2; eapply lookup_singleton_Some; eauto.
+    apply map_disjoint_empty_r.
+  Qed.
+
+  Lemma emp_trivial : ⊢ (emp : monPred biInd hpropI). simpl. auto. Qed.
+
+  Global Instance affine_heap_empty : Affine (heap_ctx ∅).
+  Proof.
+    split. intro. MonPred.unseal. repeat red. intros. apply H.
+  Qed.
+
+  Lemma init_heap : ⊢ heap_ctx ∅.
+  Proof.
+    split. MonPred.unseal. repeat red. intros. apply H.
+  Qed.
+
+  Lemma instance_heap : forall (P : monPred biInd hpropI) (Q : Prop), (forall tmps, P () tmps -> Q) -> (P ⊢ ⌜Q⌝).
+  Proof.
+    MonPred.unseal. intros. split. repeat red. intros.
+    eapply H. destruct i. eapply H0.
+  Qed.
+
+  Lemma soundness_pure h (Φ : Prop) : (&& h ⊢ (⌜ Φ ⌝) : monPred biInd hpropI) -> Φ.
+  Proof.
+    MonPred.unseal=> -[H]. repeat red in H.
+    pose (e := H () h). eapply e. reflexivity.
+  Qed.
+
+  Definition iProp := monPred biInd hpropI.
+
+  Lemma soundness (Φ : iProp) h : (⊢&& h -∗ Φ) -> Φ () h.
+  Proof.
+    MonPred.unseal=> -[H]. repeat red in H.
+    pose (e := H () ∅).
+    simpl in *. edestruct e.
+    - rewrite monPred_at_emp. split; auto; apply hempty_intro.
+    - repeat red. repeat split; auto.
+    - inversion_star h P.
+      inversion P1.
+      apply H1.
+      exists heap_empty; exists h.
+      inversion H2; subst. rewrite heap_union_empty_r in P; subst.
+      repeat split; auto. apply map_disjoint_empty_l. rewrite heap_union_empty_l. auto.
+  Qed.
+
+  Lemma completeness (Φ : iProp) h : Φ () h -> (⊢&& h -∗ Φ).
+  Proof.
+    MonPred.unseal. split. MonPred.unseal. simpl. repeat red. intros. exists emp. exists x; exists heap_empty.
+    repeat split; auto with heap_scope.
+    intros h0 P0. inversion_star h P. simpl in *. rewrite <- P2 in *. inversion P1.
+    subst. rewrite heap_union_empty_l. rewrite <- P2. destruct a. apply H.
+    apply map_disjoint_empty_r.
+  Qed.
+
+  Lemma equivalence (Φ : iProp) h : Φ () h <-> (⊢&& h -∗ Φ).
+  Proof.
+    split.
+    apply completeness.
+    apply soundness.
+  Qed.
+
+  Lemma heap_ctx_split (h h' : heap) : h ##ₘ h' -> (⊢&& (h \u h') -∗ && h ∗ && h').
+  Proof.
+    MonPred.unseal. split. MonPred.unseal. repeat red.
+    intros. exists hempty. inversion H0; subst.
+    exists heap_empty; exists heap_empty. repeat split; auto.
+    + repeat intro. inversion_star h P. inversion P1. subst.
+      exists h; exists h'. repeat split; auto. inversion P0; subst.
+      rewrite heap_union_empty_l. reflexivity.
+    + rewrite heap_union_empty_l. reflexivity.
+  Qed.
+
+  Lemma heap_ctx_split_sing (h : heap) l : h ##ₘ ({[l := tt]}) ->
+                                             (⊢&& (<[l := tt]>h) -∗ && h ∗ & l).
+  Proof.
+    iIntros (?) "HA". rewrite insert_union_singleton_r; auto. iApply heap_ctx_split; auto.
+    rewrite <- map_disjoint_singleton_r. eauto.
+  Qed.
+
+End hprop.
+
+Notation "'heap_empty'" := (∅ : heap).
+
+Notation "'\[]'" := (hempty) (at level 0).
+
+Notation "\[ P ]" := (hpure P) (at level 0, P at level 99, format "\[ P ]").
+
+Notation "H1 '\*' H2" := (hstar H1 H2) (at level 41, right associativity).
+
+Notation "\Top" := htop.
+
+
+Declare Scope heap_scope.
+
+Global Hint Resolve heap_union_empty_l heap_union_empty_r hempty_intro map_disjoint_empty_l map_disjoint_empty_r heap_union_assoc heap_disjoint_union_r_l heap_disjoint_union_l_l heap_disjoint_union_r_r heap_disjoint_union_l_r : heap_scope.
+
+Ltac inversion_star h P :=
+  match goal with
+  | H : (_ \* _) _ |- _ =>
+    let W := fresh h in
+    let w := fresh P in
+    inversion H as (W&w);
+    let W := fresh h in
+    destruct w as (W&w);
+    do 3 (let w0 := fresh P in
+          destruct w as (w0&w))
+  end.
+
+Open Scope bi_scope.
+
+Notation "'&' l" :=
+  (single l) (at level 20).
+
+Notation "'&&' h" :=
+  (heap_ctx h) (at level 20).
